Surface/Examples/Boolean.lean
@@ -11,7 +11,7 @@ def benv : GlobalEnv := [
   -- .instDecl  "IdI" ⟨1, #(`★), 0, #(), 2, #(t`#0, t`#0), (gt`#"Id" `• t`#0) `• t`#0 ⟩ #(),
   -- .classDecl "Id" #(★, ★) [] [⟨"fd", 0, #(0), 1⟩, ⟨"bwk", 0, #(1), 0⟩] [],
 
-  -- .instDecl "EqBoolI" ⟨1, #(`★), 0, #(), 1, #(gt`#"Bool"), gt`#"Eq" `• t`#0⟩ #(("eq", λˢ[gt`#"Bool"] λˢ[gt`#"Bool"] `#0)),
+  -- .instDecl "EqBoolI" ⟨1, #(★), 0, #(), 1, #(gt#"Bool"), gt#"Eq" • t#0⟩ [("eq", λˢ[gt#"Bool"] λˢ[gt#"Bool"] `#0)],
   .classDecl "Ord" #(★) [("supOrd", "Eq", [0])] [] [("leq", ⟨0, #(), 0, #(), 0, #(), t#0 -:> (t#0 -:> gt#"Ordering")⟩)],
   .classDecl "Eq" #(★) [] [] [("eq",  ⟨0, #(), 0, #(), 0, #(), t#0 -:> (t#0 -:> gt#"Bool")⟩)],
   .data (n := 2) "Bool" ★ #(("True", ⟨0, #(), 0, #(), 0,  #(), gt#"Bool"⟩),
