Translation.lean
@@ -2,10 +2,10 @@ import Core.Ty
 -- import Surface.Ty
 
 -- import Translation.Ty
-import Translation.Term
+-- import Translation.Term
 import Translation.Global
 
 
-import Translation.Ty.Lemmas
-import Translation.Term.Lemmas
+-- import Translation.Ty.Lemmas
+-- import Translation.Term.Lemmas
 import Translation.Global.Lemmas
